more experiments

src/simp_loop/binders.lean
@@ -4,6 +4,7 @@ Released under Apache 2.0 license as described in the file LICENSE.
 Authors: Johannes Hölzl
 
 Binder elimination
+Also called 1-point rules.
 
 We assume a binder `B : p → Π (α : Sort u), (α → t) → t`, where `t` is a type depending on `p`.
 Examples:
@@ -20,6 +21,173 @@ Here ..x.. are binders, maybe also some constants which provide commutativity ru
 -/
 import simp_loop.conv
 
+#check add_left_cancel_semigroup
+
+section
+
+set_option pp.all true
+example {α β : Type} {f : β → α} {p : α → Prop} :
+  ∃a : α, ∃b : (λa:α, β) a, ∃h : a = f b, p a :=
+_
+
+end
+
+namespace simp_loop
+open conv_t tactic expr
+
+namespace exists_eq_elim
+
+meta inductive info
+| binder (v : expr) (dependent : bool) | operator (side : bool)
+
+meta def check_eq (x : expr) (deps : list expr) : expr → bool
+| `(%%l = %%r) := (l = x ∧ deps.all (λx, ¬ x.occurs r)) ∨ (r = x ∧ deps.all (λx, ¬ x.occurs l))
+| _ := ff
+
+meta structure binder_eq_elim :=
+(match_binder       : expr → tactic (expr × expr))    -- returns the bound type and body
+(adapt_rel          : conv unit → conv unit)          -- optionally adapt `eq` to `iff`
+(apply_comm         : conv unit)                      -- apply commutativity rule
+(apply_op_comm      : bool → conv unit)                      -- apply commutativity rule
+(apply_congr    {α} : (expr → conv α) → conv α) -- apply congruence rule
+(apply_op_congr {α} : bool → conv α → conv α) -- apply congruence rule
+(apply_elim_eq      : conv unit)                      -- (B (x : β) (h : x = t), s x) = s t
+
+section
+parameter (b : binder_eq_elim)
+
+meta def push : list info → conv unit := λ_, skip
+/-
+| 0       := do trace "finished push", trace_lhs,
+  return ()
+| (n + 1) :=
+  (do trace ("push " ++ to_string n ++ " the current binder to the right"), trace_lhs,
+    b.apply_comm,
+    b.apply_congr $ λx, push n) <|>
+  (do trace ("push " ++ to_string n ++ " there is a dependency: switch to the right binder"), trace_lhs,
+    b.apply_congr $ λx, push n)
+-/
+
+meta def pull : list info → conv unit
+| []       := do trace "finished pull", trace_lhs,
+  b.apply_elim_eq
+| (info.binder false :: ps) := do trace "independent binder", trace_lhs,
+  b.apply_comm, b.apply_congr $ λx, pull ps
+| (info.binder true :: ps) := do trace "dependent binder", trace_lhs,
+  b.apply_congr (λe, push ps),
+  pull ps
+| (info.operator true :: ps) := do trace "operator left", trace_lhs,
+  b.congr_left (push ps),
+  pull ps
+| (info.operator true :: ps) := do trace "operator right", trace_lhs,
+  b.congr_right (push ps),
+  pull ps
+
+/-
+| [i, _] :=
+  (do trace ("pull (" ++ to_string n ++ ") the non-dependent binders to the left"), trace_lhs,
+    b.apply_comm,
+    b.apply_congr $ λx, pull n) <|>
+  (do trace ("pull (" ++ to_string n ++ ") the right (dependent binder) to the right, then try again"), trace_lhs,
+    b.apply_congr $ λe, b.push e (n + 1),
+    pull n)
+-/
+
+meta def analyse (v : expr) (deps : list expr) : expr → tactic (option $ list $ info × expr)
+| `(@Exists %%α %%p) := if check_eq v deps α then
+    return none
+  else do
+    (lam pp_n bi domain body) ← return p,
+    x ← mk_local' pp_n bi domain,
+    return [(info.binder v (deps.any $ λv, v.occurs α), body.instantiate_var x)]
+| `(%%p ∧ %%q) := do
+  return [(info.operator tt, p), (info.operator tt, q)]
+| t := return $ if check_eq v deps t then none else some []
+
+meta def find (v : expr) : list expr → expr → tactic (list info) | deps e := do
+some ps ← analyse v deps e | return [],
+ps' ← ps.mmap (λd, do
+  deps ← return $ match d with (info.binder v tt, _) := v :: deps | _ := deps end,
+  ps ← find deps d.2,
+  return $ d.1 :: ps),
+return ps'.join
+
+meta def reorder_equality : list info → conv unit | l := _
+
+meta def reorder_non_dependent1 : list info → conv (list info)
+| [] := failed
+| xs@((info.binder _ ff) :: _) := return xs
+| ((info.binder _ tt) :: xs) := do
+  xs ← b.apply_congr (λe, reorder_non_dependent1 xs),
+  b.apply_comm,
+  return xs
+| ((info.operator s) :: xs) := do
+  xs ← b.apply_op_congr s (reorder_non_dependent1 xs),
+  b.apply_op_comm s,
+  return xs
+
+meta def reorder_non_dependent : list info → conv unit | l := do
+l' ← b.apply_congr (λe, reorder_non_dependent1 l) | reorder_equality l,
+b.apply_comm,
+b.apply_congr (λe, reorder_non_dependent l')
+
+meta def run : expr → tactic unit
+| `(@Exists %%α %%p) := do
+  (lam pp_n bi domain body) ← return p,
+  v ← mk_local' pp_n bi domain,
+  let t := body.instantiate_var v,
+  ps ← find v [v] t,
+  _
+| _ := skip
+
+end
+end exists_eq_elim
+
+
+
+#exit
+
+meta structure binder_eq_elim :=
+(analyse_head : expr → tactic (expr × expr × expr × expr))
+(analyse : expr → tactic (list (expr × list expr × expr × expr)))
+
+/- `(t, v, x, t') ∈ analyse_head e` splits e s.t. e = t[x := λv. t'] -/
+/- `(t, vs, x, t') ∈ analyse e` splits e s.t. e = t[x := λvs. t'] -/
+
+namespace binder_eq_elim
+
+protected meta def check_eq (b : binder_eq_elim) (x : expr) : expr → bool
+| `(%%l = %%r) := ((l = x ∧ ¬ x.occurs r) ∨ (r = x ∧ ¬ x.occurs l))
+| _ := ff
+
+protected meta def eliminate (b : binder_eq_elim) (v : expr) :
+  expr → list (expr × list expr × expr × expr) → tactic expr :=
+_
+
+
+protected meta def find (b : binder_eq_elim) (x : expr) :
+  expr → tactic (list $ list $ expr × list expr × expr × expr) | e := do
+ps ← b.analyse e,
+ps' ← ps.mmap (λd, do
+  ⟨t, vs, v, t'⟩ ← return d,
+  if vs.any (b.check_eq x) ∨ b.check_eq x t' then
+    return []
+  else do
+    ps' ← find t',
+    return $ ps'.map (λl, d :: l)),
+return ps'.join
+
+protected meta def run (b : binder_eq_elim) (e : expr) : tactic expr := do
+(t, v, x, t') ← b.analyse_head e,
+ps ← b.find v t',
+ps.mfirst (b.eliminate v t')
+
+end binder_eq_elim
+
+
+#exit
+
+
 namespace simp_loop
 open conv_t tactic expr
 
@@ -32,9 +200,9 @@ meta structure binder_eq_elim :=
 
 namespace binder_eq_elim
 
-protected meta def check_eq (b : binder_eq_elim) (x : expr) : expr → tactic unit
-| `(@eq %%β %%l %%r) := guard ((l = x ∧ ¬ x.occurs r) ∨ (r = x ∧ ¬ x.occurs l))
-| _ := fail "no match"
+protected meta def check_eq (b : binder_eq_elim) (x : expr) : expr → tactic bool
+| `(@eq %%β %%l %%r) := return ((l = x ∧ ¬ x.occurs r) ∨ (r = x ∧ ¬ x.occurs l))
+| _ := return ff
 
 protected meta def push (b : binder_eq_elim) (x : expr) : ℕ → conv unit
 | 0       := do trace "finished push", trace_lhs,
@@ -57,37 +225,53 @@ protected meta def pull (b : binder_eq_elim) : ℕ → conv unit
     b.apply_congr $ λe, b.push e (n + 1),
     pull n)
 
-protected meta def check (b : binder_eq_elim) (x : expr) : ℕ → expr → tactic ℕ
+/-- `b.find x n e` looks for a binder in the binder-prefix of `e`, where a equality on `x` is bound.
+It returns all occurrences of equalitie under binders, to each occurence `n` is added.
+
+TODO: Maybe the list of occurences is not necessary. We can check at each equality if the
+other side depends on `x`. Reason: everything needs to be parameterized in `x`, either it is hidden
+using some kind of relation, or it appears explicitly.
+
+Can we already decide by looking at the binder type if we should push or pull?
+-/
+protected meta def find (b : binder_eq_elim) (x : expr) : ℕ → expr → tactic (list ℕ)
 | i e := do
-  (β, f) ← b.match_binder e,
-  (b.check_eq x β >> return i)
-  <|> (do
-    (lam n bi d bd) ← return f,
+  some (β, f) ← try_core $ b.match_binder e | return [],
+  b ← b.check_eq x β,
+  is ← (do
+    (lam n bi d bd) ← return f | return [],
     x ← mk_local' n bi d,
-    check (i + 1) (bd.instantiate_var x))
+    find (i + 1) (bd.instantiate_var x)),
+  return (if b then i :: is else is)
 
 protected meta def conv (b : binder_eq_elim) : conv unit := do
   (β, f) ← lhs >>= (lift_tactic ∘ b.match_binder),
   (lam n bi d bd) ← return f,
   x ← mk_local' n bi d,
-  i ← b.check x 0 (bd.instantiate_var x),
-  b.adapt_rel (b.pull i)
-
-
+  is ← b.find x 0 (bd.instantiate_var x),
+  is.mfirst (b.adapt_rel ∘ b.pull)
 
 end binder_eq_elim
 
 section exists_eq_elim
 
-theorem {u v} exists_comm {α : Sort u} {β : Sort v} (p : α → β → Prop) :
+theorem exists_and_distrib_left {α : Sort*} (p : α → Prop) (q : Prop) :
+  (∃a, p a ∧ q) ↔ (∃a, p a) ∧ q :=
+⟨λ⟨a, hp, hq⟩, ⟨⟨a, hp⟩, hq⟩, λ ⟨⟨a, hp⟩, hq⟩, ⟨a, hp, hq⟩⟩
+
+theorem exists_and_distrib_right {α : Sort*} (p : α → Prop) (q : Prop) :
+  (∃a, q ∧ p a) ↔ q ∧ (∃a, p a) :=
+⟨λ⟨a, hq, hp⟩, ⟨hq, ⟨a, hp⟩⟩, λ ⟨hq, ⟨a, hp⟩⟩, ⟨a, hq, hp⟩⟩
+
+theorem exists_comm {α : Sort*} {β : Sort*} (p : α → β → Prop) :
   (∃a b, p a b) ↔ (∃b a, p a b) :=
 ⟨λ⟨a, ⟨b, h⟩⟩, ⟨b, ⟨a, h⟩⟩, λ⟨a, ⟨b, h⟩⟩, ⟨b, ⟨a, h⟩⟩⟩
 
-theorem {u v} exists_elim_eq_left {α : Sort u} (a : α) (p : Π(a':α), a' = a → Prop) :
+theorem exists_elim_eq_left {α : Sort*} (a : α) (p : Π(a':α), a' = a → Prop) :
   (∃(a':α) (h : a' = a), p a' h) ↔ p a rfl :=
 ⟨λ⟨a', ⟨h, p_h⟩⟩, match a', h, p_h with ._, rfl, h := h end, λh, ⟨a, rfl, h⟩⟩
 
-theorem {u v} exists_elim_eq_right {α : Sort u} (a : α) (p : Π(a':α), a = a' → Prop) :
+theorem exists_elim_eq_right {α : Sort*} (a : α) (p : Π(a':α), a = a' → Prop) :
   (∃(a':α) (h : a = a'), p a' h) ↔ p a rfl :=
 ⟨λ⟨a', ⟨h, p_h⟩⟩, match a', h, p_h with ._, rfl, h := h end, λh, ⟨a, rfl, h⟩⟩
 
@@ -102,15 +286,15 @@ end exists_eq_elim
 
 section forall_eq_elim
 
-theorem {u v} forall_comm {α : Sort u} {β : Sort v} (p : α → β → Prop) :
+theorem forall_comm {α : Sort*} {β : Sort*} (p : α → β → Prop) :
   (∀a b, p a b) ↔ (∀b a, p a b) :=
 ⟨assume h b a, h a b, assume h b a, h a b⟩
 
-theorem {u v} forall_elim_eq_left {α : Sort u} (a : α) (p : Π(a':α), a' = a → Prop) :
+theorem forall_elim_eq_left {α : Sort*} (a : α) (p : Π(a':α), a' = a → Prop) :
   (∀(a':α)(h : a' = a), p a' h) ↔ p a rfl :=
 ⟨λh, h a rfl, λh a' h_eq, match a', h_eq with ._, rfl := h end⟩
 
-theorem {u v} forall_elim_eq_right {α : Sort u} (a : α) (p : Π(a':α), a = a' → Prop) :
+theorem forall_elim_eq_right {α : Sort*} (a : α) (p : Π(a':α), a = a' → Prop) :
   (∀(a':α)(h : a = a'), p a' h) ↔ p a rfl :=
 ⟨λh, h a rfl, λh a' h_eq, match a', h_eq with ._, rfl := h end⟩
 
@@ -125,8 +309,7 @@ end forall_eq_elim
 
 section test
 
-universes u v w w₂
-variables {α : Type u} {β : Type v} {ι : Sort w} {ι₂ : Sort w₂} {a : α} {γ : β → Type} {δ : α → Type}
+variables {α : Type*} {β : Type*} {ι : Sort*} {ι₂ : Sort*} {a : α} {γ : β → Type*} {δ : α → Type*}
   {f : α → β} {p : β → Prop}
 
 example : (∃b, ∃c:γ b, ∃h : f a = b, p b) ↔ (∃c:γ (f a), p (f a)) :=
@@ -153,6 +336,10 @@ by conversion exists_eq_elim.conv
 
 example {f : Πa, δ a → β} :
   (∃b, ∃a, ∃d:δ a, ∃h' : a = a ∧ b = b, ∃h : f a d = b, ∃c:γ b, p b) ↔ _ :=
+by conversion exists_eq_elim.conv
+
+example {f : α → β} {q : β → α → Prop} :
+  (∃b, ∃a, ∃h:q b a, ∃h' : b = b, ∃h : f a = b, ∃c:γ b, p b) ↔ _ :=
 by conversion exists_eq_elim.conv
 
 end test
